Cleanup current proofs

MECMAR/props/Correctness.v
@@ -1,5 +1,5 @@
 From Coq Require Import PeanoNat ZArith Bool Lia Program.Equality.
-From Warblre Require Import Tactics Focus Result Base Patterns StaticSemantics Notation Semantics.
+From Warblre Require Import Tactics Specialize Focus Result Base Patterns StaticSemantics Notation Semantics.
 
 Import Result.Notations.
 
@@ -10,165 +10,136 @@ Module Correctness.
 
   Create HintDb warblre.
 
-  Notation "x '[@' n ']'" := (match_state (MatchState.input x) n (MatchState.captures x)) (at level 50, left associativity).
-  Notation "x '[$' c ']'" := (match_state (MatchState.input x) (MatchState.endIndex x) c) (at level 50, left associativity).
-  Notation "x '[@' n '$' c ']'" := (match_state (MatchState.input x) n c) (at level 50, left associativity).
+  Ltac Zhelper := repeat
+  (   hypotheses_reflector
+  ||  goal_reflector
+  ||  normalize_Z_comp
+  ||  spec_reflector Z.leb_spec0
+  ||  spec_reflector Z.ltb_spec0).
+
+  Notation "s '[@' n '$' c ']'" := (match_state s n c) (at level 50, left associativity).
 
   Inductive directionalProgress: direction -> MatchState -> MatchState -> Prop :=
   | dpForward: forall x y, (MatchState.endIndex x <= MatchState.endIndex y)%Z -> directionalProgress forward x y
-  | dpBackward: forall x y, (MatchState.endIndex x >= MatchState.endIndex y)%Z -> directionalProgress backward x y
-  .
-  #[export]
-  Hint Constructors directionalProgress : core.
+  | dpBackward: forall x y, (MatchState.endIndex x >= MatchState.endIndex y)%Z -> directionalProgress backward x y.
 
   Inductive progress: direction -> MatchState -> MatchResult -> Prop :=
   | pStep: forall dir x y, 
       (MatchState.input x) = (MatchState.input y)
     -> directionalProgress dir x y
     -> progress dir x (Success y)
-  | pFail: forall dir x f, progress dir x (Failure f)
-  .
+  | pFail: forall dir x f, progress dir x (Failure f).
   #[export]
-  Hint Constructors progress : core.
+  Hint Constructors progress: core.
 
-  Ltac destruct_dps := repeat lazymatch goal with
-  | [ H: directionalProgress ?d _ _ |- _ ] => is_constructor d; inversion H; clear H
-  end.
-
-  Ltac saturate_transitive rel trans := repeat match goal with
-  | [ R1: rel ?S ?T, R2: rel ?T ?U |- _ ] => lazymatch goal with
-    |  [ _ : rel S U |- _ ] => fail
-    | [ |- _ ] => pose proof (trans S T U R1 R2)
-    end
-  end; try assumption.
-
+  Definition OnInput (x: MatchState) (str: list Character) := MatchState.input x = str.
+  Definition Valid (x: MatchState) := (0 <= MatchState.endIndex x <= Z.of_nat (length (MatchState.input x)))%Z.
   Module MatchState.
-    Lemma reconstruction: forall x, x = match_state (MatchState.input x) (MatchState.endIndex x) (MatchState.captures x).
-    Proof. destruct x. reflexivity. Qed.
-
-    Lemma id: forall x, x [@ MatchState.endIndex x ] = x.
-    Proof. intros. destruct x; reflexivity. Qed.
-
-    Lemma normalize: forall x e c, x [$ c] [@ e] = x [@ e] [$ c].
-    Proof. intros. destruct x; reflexivity. Qed.
+    Ltac normalize := repeat
+    (   simpl (match_state _ _ _) in *
+    ||  lazymatch goal with
+        | [ x: MatchState |- _ ] =>
+          let input := fresh "input_" x in
+          let endIndex := fresh "endIndex_" x in
+          let captures := fresh "captures_" x in
+          destruct x as [ input endIndex captures ]
+        | [ H: OnInput (match_state ?input _ _) ?str |- _ ] =>
+          unfold OnInput in H; cbn in H;
+          try rewrite -> H in *; clear H; clear input
+        end).
   End MatchState.
 
   Module Progress.
+    Local Ltac hammer :=
+      repeat match goal with
+      | [ H: progress _ _ (Success _) |- _ ] => inversion H; clear H; subst
+      | [ H: directionalProgress ?d _ _ |- _ ] => is_constructor d; inversion H; clear H
+      | [ _: directionalProgress ?d _ _ |- _ ] => destruct d
+      | [ |- progress _ _ ?y ] => is_var y; let Eq := fresh "Eq" y in destruct y eqn:Eq
+      | [ |- progress ?d _ _ ] => is_constructor d; constructor
+      | [ |- progress ?d _ _ ] => destruct d
+      | [ |- directionalProgress ?d _ _ ] => is_constructor d; constructor
+      | [ |- directionalProgress ?d _ _ ] => destruct d
+      end.
+
     Lemma refl: forall dir x, (progress dir) x (Success x).
-    Proof. intros. destruct dir; constructor; try reflexivity; constructor; normalize_Z_comp; apply Z.le_refl. Qed.
+    Proof. intros. hammer. 1,3: congruence. all: lia. Qed.
 
     Lemma trans: forall dir x y z, (progress dir) x (Success y) -> (progress dir) y z -> (progress dir) x z.
     Proof.
-      intros.
-      repeat match goal with
-      | [ H: (progress _) _ (Success _) |- _ ] => inversion H; clear H; subst
-
-      | [ |- (progress _) _ ?y ] => is_var y; let Eq := fresh "Eq" y in destruct y eqn:Eq
-      | [ |- (progress _) _ ?y ] => constructor
-      end.
-      - congruence.
-      - destruct dir; destruct_dps; constructor; normalize_Z_comp; saturate_transitive Z.le Z.le_trans.
+      intros. hammer.
+      1,3: congruence.
+      all: lia.
     Qed.
 
-    Lemma restate: forall dir x y,
-          (progress dir) x (Success y)
-      ->  (progress dir) x (Success (x [@ MatchState.endIndex y])).
+    Lemma ignores_captures_r: forall c1 c2 dir x i n,
+          (progress dir) x (Success (i [@ n $ c1]))
+      <-> (progress dir) x (Success (i [@ n $ c2])).
     Proof.
-      intros. inversion H. constructor; simpl in *.
-      - reflexivity.
-      - destruct dir; destruct_dps; constructor; assumption.
+      intros; split; intros; hammer; subst.
+      all: try assumption.
+      all: cbn in *; lia.
     Qed.
 
-    Lemma ignores_captures: forall dir x y cx cy,
-          (progress dir) x (Success y) 
-      ->  (progress dir) 
-            (match_state (MatchState.input x) (MatchState.endIndex x) cx)
-            (Success (match_state (MatchState.input y) (MatchState.endIndex y) cy)).
+    Lemma ignores_captures_l: forall c1 c2 dir i n y,
+          (progress dir) (i [@ n $ c1]) (Success y)
+      <-> (progress dir) (i [@ n $ c2]) (Success y).
     Proof.
-      intros. inversion H. constructor; simpl.
-      - assumption.
-      - destruct dir; destruct_dps; constructor; assumption.
+      intros; split; intros; hammer; subst.
+      all: try assumption.
+      all: cbn in *; lia.
     Qed.
 
-    Lemma ignores_captures_r: forall dir x n c,
-          (progress dir) x (Success (x [@ n $ c]))
-      <->  (progress dir) x (Success (x [@ n])).
-    Proof.
-      intros; split; intros; inversion H; constructor; simpl.
-      - assumption.
-      - destruct dir; destruct_dps; constructor; assumption.
-      - reflexivity.
-      - destruct dir; destruct_dps; constructor; assumption.
-    Qed.
+    Lemma progress_same_input: forall dir x y, progress dir x (Success y)
+      -> MatchState.input x = MatchState.input y.
+    Proof. intros. inversion H. assumption. Qed.
 
-    Lemma ignores_captures_l: forall dir x n c,
-          (progress dir) (x [@ n $ c]) (Success x)
-      <->  (progress dir) (x [@ n]) (Success x).
-    Proof.
-      intros; split; intros; inversion H; constructor; simpl.
-      - assumption.
-      - destruct dir; destruct_dps; constructor; assumption.
-      - reflexivity.
-      - destruct dir; destruct_dps; constructor; assumption.
-    Qed.
-
-    Lemma simplify_l: forall dir x y c, progress dir (x [$ c]) (Success y) <-> progress dir x (Success y).
-    Proof.
-      intros; split; intros; inversion H; constructor; simpl.
-      - assumption.
-      - destruct dir; destruct_dps; constructor; assumption.
-      - assumption.
-      - destruct dir; destruct_dps; constructor; assumption.
-    Qed.
-
-    Lemma simplify_r: forall dir x y c, progress dir x (Success (y [$ c])) <-> progress dir x (Success y).
-    Proof.
-      intros; split; intros; inversion H; constructor; simpl.
-      - assumption.
-      - destruct dir; destruct_dps; constructor; assumption.
-      - assumption.
-      - destruct dir; destruct_dps; constructor; assumption.
-    Qed.
-    
-    Lemma normalize: forall dir x y, progress dir x (Success y) -> y = (x [@ MatchState.endIndex y] [$ MatchState.captures y]).
-    Proof. intros. inversion H. destruct y. cbn in *. subst. reflexivity. Qed.
-
-    Ltac clean := repeat
-    (   rewrite -> MatchState.id in *
-    ||  rewrite -> MatchState.normalize in *
-    ||  rewrite -> Progress.ignores_captures_r in *
-    ||  rewrite -> Progress.simplify_l in *
-    ||  rewrite -> Progress.simplify_r in *
+    Ltac normalize := repeat (
+        MatchState.normalize
+    ||  rewrite <- (ignores_captures_l (DMap.empty _)) in *
+    ||  rewrite <- (ignores_captures_r (DMap.empty _)) in *
     ||  lazymatch goal with
-        | [ H: progress _ ?x (Success (?x [@ _ ] [$ _ ])) |- _ ] => fail
-        | [ H: progress _ ?x (Success ?y) |- _ ] =>
-          let Eq := fresh "Eq" x y in
-          pose proof normalize _ _ _ H as Eq;
-          rewrite -> Eq in *
+        | [ H: progress _ (?i [@ _ $ _]) (Success (?i [@ _ $ _])) |- _ ] => fail
+        | [ H: progress _ (?i1 [@ _ $ _]) (Success (?i2 [@ _ $ _])) |- _ ] =>
+          let Tmp := fresh in
+          pose proof progress_same_input as Tmp;
+          specialize Tmp with (1 := H);
+          cbn in Tmp;
+          rewrite -> Tmp in *;
+          clear Tmp
         end
-    ||  assumption).
+    ).
+
+    Local Ltac solvers := assumption || apply refl || reflexivity.
+    Ltac solve := normalize; solve [ solvers ].
+
+    Ltac saturate_step := normalize; match goal with
+    | [ H1: progress ?dir ?x (Success ?y), H2: progress ?dir ?y (Success ?z) |- _ ] =>
+      let H := fresh "ps_trans_" H1 H2 in
+      pose proof Progress.trans as H;
+      specialize H with (1 := H1) (2 := H2);
+      check_not_duplicated H
+    end.
+    Ltac saturate := repeat (normalize; saturate_step); normalize; try solvers.
   End Progress.
 
-  Ltac ignore_captures_change' x captures :=
-    apply Progress.trans with (y := (match_state (MatchState.input x) (MatchState.endIndex x) captures));
-    [ replace x with (match_state (MatchState.input x) (MatchState.endIndex x) (MatchState.captures x)) at 1 by (destruct x; reflexivity);
-      apply Progress.ignores_captures; apply Progress.refl
-    | idtac ].
-  Ltac ignore_captures_change := match goal with
-  | [ |- progress _ ?x (_ (match_state (MatchState.input ?x) (MatchState.endIndex ?x) ?captures)) ] => is_var x; ignore_captures_change' x captures
-  | [ |- progress _ ?x (_ (match_state (MatchState.input ?x) (MatchState.endIndex ?x) ?captures) _) ] => is_var x; ignore_captures_change' x captures
-  end.
-
-  Definition OnInput (x: MatchState) (str: list Character) := MatchState.input x = str.
-  Definition MonotonousContinuation (dir: direction) (str: list Character) (c: MatcherContinuation) := forall x, OnInput x str -> (progress dir) x (c x).
-  Definition MonotonousMatcher (dir: direction) (str: list Character) (m: Matcher) := forall x c, OnInput x str -> (MonotonousContinuation dir str) c -> (progress dir) x (m x c).
-  #[export]
-  Hint Transparent MonotonousContinuation MonotonousMatcher : core.
-
   Module Monotony.
-    Lemma matcher_to_continuation: forall dir str m c, MonotonousMatcher dir str m -> MonotonousContinuation dir str c 
+    Definition MonotonousContinuation (dir: direction) (str: list Character) (c: MatcherContinuation) := forall x, OnInput x str -> (progress dir) x (c x).
+    Definition MonotonousMatcher (dir: direction) (str: list Character) (m: Matcher) := 
+      forall x c, OnInput x str -> MonotonousContinuation dir str c -> (progress dir) x (m x c).
+
+    Lemma matcher_to_continuation: forall dir str m c, MonotonousMatcher dir str m -> MonotonousContinuation dir str c
       -> MonotonousContinuation dir str (fun (x: MatchState) => m x c).
     Proof. intros. unfold MonotonousContinuation. intros. apply H; assumption. Qed.
+
+    Ltac check_type t T := lazymatch type of t with
+    | T => idtac
+    | _ => fail
+    end.
+    Ltac obvious_transitivity := match goal with
+      | [ |- progress _ _ (?m ?y' _) ] => check_type m Matcher; apply Progress.trans with (y := y')
+      | [ |- progress _ _ (?c ?y') ] => check_type c MatcherContinuation; apply Progress.trans with (y := y')
+      end.
 
     Lemma repeatMatcher: forall fuel dir str x m min max greedy c groupsWithin,
               MonotonousMatcher dir str m
@@ -176,158 +147,79 @@ Module Correctness.
           ->  OnInput x str
           ->  progress dir x (repeatMatcher' m min max greedy x c groupsWithin fuel).
     Proof.
-      induction fuel; intros; delta repeatMatcher'; try constructor.
-      cbn.
-      repeat match goal with
-      | [ |- (progress _) _ (if ?b then _ else _) ] => destruct b
-      end; try solve
-      [ apply H0; assumption
-      | ignore_captures_change; apply H;
-        [ assumption
-        | delta MonotonousContinuation; cbn; intros;
-          repeat match goal with
-          | [ |- (progress _) _ (if ?b then _ else _) ] => destruct b
-          end; try (now constructor);
-          apply IHfuel with (str := str); assumption ] ].
+      induction fuel; try constructor.
+      intros. cbn.
+      focus § _ _ _ [] § auto destruct.
+      - apply H0; assumption.
+      - obvious_transitivity; [ Progress.solve | ].
+        apply H; try assumption.
+        cbn. intros x' OIx'. focus § _ _ _ [] § auto destruct; try easy.
+        apply IHfuel with (str := str); assumption.
+      - apply H0; assumption.
+      - obvious_transitivity; [ Progress.solve | ].
+        apply H; try assumption.
+        cbn. intros x' OIx'. focus § _ _ _ [] § auto destruct; try easy.
+        apply IHfuel with (str := str); assumption.
+      - obvious_transitivity; [ Progress.solve | ].
+        apply H; try assumption.
+        cbn. intros x' OIx'. focus § _ _ _ [] § auto destruct; try easy.
+        apply IHfuel with (str := str); assumption.
+      - apply H0; assumption.
     Qed.
 
-    Lemma compileSubpattern: forall r rer dir str, MonotonousMatcher dir str (compileSubPattern r rer dir).
+    Lemma compileSubPattern: forall r rer dir str, MonotonousMatcher dir str (compileSubPattern r rer dir).
     Proof.
-      induction r.
-      - delta MonotonousMatcher. cbn. intros.
-        repeat match goal with
-        | [ |- (progress _) _ (if ?b then _ else _) ] => destruct b
-        | [ |- (progress _) _ (match ?b with | _ => _ end) ] => destruct b
-        end; try now constructor.
+      induction r; intros; intros x c OIx Mc; cbn.
+      - focus § _ _ _ []§ auto destruct; try easy.
         destruct dir;
-          (lazymatch goal with [ |- progress _ _ (_ ?x') ] => apply Progress.trans with (y := x') end;
-          [ constructor; [ reflexivity | constructor; simpl; lia ]
-          | apply H0; inversion H; subst; reflexivity ]).
-      - delta MonotonousMatcher. cbn. intros.
-        repeat match goal with
-        | [ |- (progress _) _ (if ?b then _ else _) ] => destruct b
-        | [ |- (progress _) _ (match ?b with | _ => _ end) ] => destruct b
-        end; (apply IHr1 with (str := str) + apply IHr2 with (str := str)); assumption.
-      - delta MonotonousMatcher. cbn. intros.
-        apply Monotony.repeatMatcher with (str := str); try assumption.
+          (obvious_transitivity;
+          [ constructor; [ reflexivity | constructor; cbn; lia ]
+          | apply Mc; inversion OIx; subst; reflexivity ]).
+      - focus § _ _ _ []§ auto destruct; (apply IHr1 with (str := str) + apply IHr2 with (str := str)); assumption.
+      - apply Monotony.repeatMatcher with (str := str); try assumption.
         apply IHr.
-      - (* Pesky case which doesn't start like the others *)
-        intros. cbn.
-        repeat lazymatch goal with
-        | [ |- MonotonousMatcher _ _ (if ?b then _ else _) ] => destruct b
-        end; delta MonotonousMatcher; cbn; intros;
-          [ apply IHr1 with (str := str) | apply IHr2 with (str := str) ]; try apply matcher_to_continuation; auto.
-      - delta MonotonousMatcher. cbn. intros.
-        specialize (IHr rer dir). delta MonotonousMatcher in IHr. cbn in IHr.
-        apply IHr with (str := str); try assumption. delta MonotonousContinuation. cbn. intros.
-        repeat match goal with
-        | [ |- (progress _) _ (if ?b then _ else _) ] => destruct b
-        | [ |- (progress _) _ (match ?b with | _ => _ end) ] => destruct b
-        end; try now constructor.
-        delta MonotonousContinuation in H.
-        inversion H; inversion H1. subst. rewrite <- H3.
-        delta MonotonousContinuation in H0. cbn in H0.
-        ignore_captures_change.
-        apply H0. rewrite <- H3. reflexivity.
-      - delta MonotonousMatcher. cbn. intros.
-        repeat match goal with
-        | [ |- (progress _) _ (if ?b then _ else _) ] => destruct b
-        | [ |- (progress _) _ (match ?b with | _ => _ end) ] => destruct b
-        end; try now constructor.
-        ignore_captures_change. apply H0. assumption.
+      - focus § _ _ _ []§ auto destruct.
+        + apply IHr1 with (str := str); try assumption.
+          intros x' OIx'.
+          apply IHr2 with (str := str); try assumption.
+        + apply IHr2 with (str := str); try assumption.
+          intros x' OIx'.
+          apply IHr1 with (str := str); try assumption.
+      - apply IHr with (str := str); try assumption. cbn. intros x' OIx'.
+        focus § _ _ _ []§ auto destruct; try easy.
+        Progress.normalize.
+        obvious_transitivity.
+        + Progress.solve.
+        + apply Mc. Progress.solve.
+      - focus § _ _ _ []§ auto destruct; try easy.
+        obvious_transitivity.
+        + Progress.solve.
+        + apply Mc. Progress.solve.
+      Qed.
+
+      Lemma compilePattern: forall r rer input i, progress forward (match_state input (Z.of_nat i) (DMap.empty CaptureRange)) (compilePattern r rer input i).
+      Proof.
+        intros. delta compilePattern. cbn.
+        remember (match_state input (Z.of_nat i) (DMap.empty CaptureRange)) as x.
+        focus § _ _ _ [] § auto destruct.
+        - pose proof compileSubPattern. unfold MonotonousMatcher in H.
+          apply H with (str := input).
+          + subst. reflexivity.
+          + intros y OIy. apply Progress.refl.
+        - constructor.
       Qed.
   End Monotony.
-
-
-  Lemma ZofNat_is_pos: forall n, (0 <= Z.of_nat n)%Z.
-  Proof. induction n; lia. Qed.
-
-  Ltac ztac := repeat match goal with
-  | [ H: context[ Z.min ?x ?y] |- _ ] =>
-      ( ( assert(x <= y)%Z by lia; replace (Z.min x y) with x in * by (symmetry; apply Z.min_l; assumption) )
-      + ( assert(y <= x)%Z by lia; replace (Z.min x y) with y in * by (symmetry; apply Z.min_r; assumption) ) )
-  | [ H: context[ Z.of_nat ?n ] |- _ ] => lazymatch goal with
-    | [ _: (0 <= Z.of_nat n)%Z |- _ ] => fail
-    | [ |- _ ] => pose proof (ZofNat_is_pos n)
-    end
-  end.
-
-  Ltac check_not_duplicated H :=
-    let T := type of H in
-    lazymatch goal with
-    | [ _: T, _: T |- _ ] => fail
-    | [ |- _ ] => idtac
-    end.
-
-  Ltac saturate_progress_step dir := match goal with
-  | [ H1: progress dir ?x (Success ?y), H2: progress ?dir ?y (Success ?z) |- _ ] =>
-    let H := fresh "sp_trans_" H1 H2 in
-    pose proof Progress.trans as H;
-    specialize H with (1 := H1) (2 := H2);
-    check_not_duplicated H
-  | [ H1: ?input = MatchState.input ?x,
-      H2: ?endIndex = MatchState.endIndex ?x,
-      H3: ?y = match_state ?input ?end_index ?c
-    |- _ ] => let H := fresh "sp_change_" x y in
-              pose proof (Progress.refl dir x) as H;
-              apply Progress.ignores_captures with (cx := MatchState.captures x) (cy := c) in H;
-              rewrite <- MatchState.reconstruction in H;
-              rewrite <- H1 in H;
-              rewrite <- H2 in H;
-              rewrite <- H3 in H;
-              check_not_duplicated H
-  end.
-  Ltac saturate_progress dir := repeat saturate_progress_step dir.
-
-  Notation "'validState' x" := (0 <= MatchState.endIndex x <= Z.of_nat (length (MatchState.input x)))%Z (at level 99).
-
-  Ltac auto_destruct t := lazymatch t with
-  | match ?c with | _ => _ end => let Eq := fresh "MatchEq_" in destruct c eqn:Eq
-  | if ?c then _ else _ => let Eq := fresh "IfEq_" in destruct c eqn:Eq
-  | ?l _ => auto_destruct l
-  end; try discriminate.
-
-  Tactic Notation "focus" constr(f) "auto" "destruct" := (
-    assert_type f focus;
-    repeat(
-      let g := focus_get_goal in
-      let t := focus_excise f g in
-      auto_destruct t)).
-
-  Tactic Notation "focus" constr(f) "auto" "destruct" "in" hyp(H) := (
-    assert_type f focus;
-    repeat(
-      let g := focus_get_hypothesis H in
-      let t := focus_excise f g in
-      auto_destruct t)).
 
   Ltac step_progress := match goal with
   | [ |- progress ?dir _ _ ] => is_constructor dir; constructor; [ reflexivity | constructor; cbn; lia ]
   | [ |- progress ?dir _ _ ] => destruct dir; step_progress
   end.
 
-  Inductive Specialized {A B: Type} (a: A) (b: B) :=
-  | AlreadySpecialized: Specialized a b.
-  Ltac auto_specialize := repeat match goal with
-  | [ a: _, b: _ |- _ ] => lazymatch goal with
-    | [ _: Specialized a b |- _ ] => fail
-    | [ |- _ ] =>
-      pose proof (AlreadySpecialized a b);
-      let H := fresh a b in
-      pose proof a as H;
-      specialize H with (1 := b)
-    end
-  end.
-
-  Ltac specialize_once := match goal with
-  | [ H: _, H': _ |- _ ] => specialize H with (1 := H')
-  end.
-
   Module IntermediateValue.
     Ltac search := try assumption; match goal with
       | [ H: ?c ?y = Success ?z |- exists x, _ /\ ?c x = Success ?z ] => exists y; split; [ try assumption | apply H ]
       end; match goal with
-      | [ |- progress ?dir _ _ ] => saturate_progress dir; try assumption
+      | [ |- progress ?dir _ _ ] => Progress.saturate
       end.
 
     Lemma repeatMatcher: forall fuel dir x m min max greedy c groupsWithin z,
@@ -338,21 +230,21 @@ Module Correctness.
       induction fuel; deltaf repeatMatcher'; cbn; intros;
         focus § _ [] _ § auto destruct in H.
       - discriminate.
-      - IntermediateValue.search. apply Progress.refl.
+      - IntermediateValue.search.
       - auto_specialize; Coq.Program.Tactics.destruct_conjs.
         focus § _ [] _ § auto destruct in H3.
         auto_specialize; Coq.Program.Tactics.destruct_conjs.
-        IntermediateValue.search. Progress.clean.
-      - IntermediateValue.search. apply Progress.refl.
+        IntermediateValue.search.
+      - IntermediateValue.search.
       - auto_specialize; Coq.Program.Tactics.destruct_conjs.
         focus § _ [] _ § auto destruct in H3.
         auto_specialize; Coq.Program.Tactics.destruct_conjs.
-        IntermediateValue.search. Progress.clean.
+        IntermediateValue.search.
       - auto_specialize; Coq.Program.Tactics.destruct_conjs.
         focus § _ [] _ § auto destruct in H3.
         auto_specialize; Coq.Program.Tactics.destruct_conjs.
-        IntermediateValue.search. Progress.clean.
-      - IntermediateValue.search. apply Progress.refl.
+        IntermediateValue.search.
+      - IntermediateValue.search.
     Qed.
 
     Lemma compileSubPattern: forall r rer dir x c z, (compileSubPattern r rer dir) x c = Success z 
@@ -368,77 +260,75 @@ Module Correctness.
       + repeat (specialize_once; Coq.Program.Tactics.destruct_conjs). IntermediateValue.search.
       + repeat (specialize_once; Coq.Program.Tactics.destruct_conjs). IntermediateValue.search.
       + specialize IHr with (1 := H). Coq.Program.Tactics.destruct_conjs.
-        focus §_ [] _§ auto destruct in H1. IntermediateValue.search. Progress.clean.
-      + IntermediateValue.search. Progress.clean. apply Progress.refl.
+        focus §_ [] _§ auto destruct in H1. IntermediateValue.search.
+      + IntermediateValue.search.
     Qed.
   End IntermediateValue.
 
   Module Safety.
-    Notation "'SafeContinuation' x '|' dir '|' c" := (forall x', validState x' -> progress dir x (Success x') -> c x' <> assertion_failed) 
-      (x at level 0, dir at level 0, c at level 0, at level 99).
-    Notation "'SafeMatcher' dir '|' m" := (forall x c,
-          validState x
-      ->  (SafeContinuation x | dir | c)
-      ->  m x c <> assertion_failed)
-      (dir at level 0, m at level 0, at level 99).
+    Definition SafeContinuation (x: MatchState) (dir: direction) (c: MatcherContinuation) := (forall x', Valid x' -> progress dir x (Success x') -> c x' <> assertion_failed).
+    Definition SafeMatcher (dir: direction) (m: Matcher) := (forall x c,
+          Valid x
+      ->  (SafeContinuation x dir c)
+      ->  m x c <> assertion_failed).
 
     Lemma continuation_weakening: forall x x' dir (c: MatcherContinuation), progress dir x (Success x')
-      -> SafeContinuation x | dir | c -> SafeContinuation x' | dir | c.
-    Proof. intros. apply H0; try assumption. saturate_progress dir. assumption. Qed.
+      -> SafeContinuation x dir c -> SafeContinuation x' dir c.
+    Proof. intros. intros y Vy Pxy. apply H0; try assumption. Progress.saturate. Qed.
 
     Lemma repeatMatcher: forall fuel dir m min max greedy captures,
-      SafeMatcher dir | m -> SafeMatcher dir | (fun x c => repeatMatcher' m min max greedy x c captures fuel).
+      SafeMatcher dir m -> SafeMatcher dir (fun x c => repeatMatcher' m min max greedy x c captures fuel).
     Proof.
-      induction fuel; intros; cbn; try easy.
+      induction fuel; intros; intros x c Vx Sc; cbn; try easy.
       focus § _ (_ [] _) § auto destruct.
-      - apply H1; try assumption. apply Progress.refl.
-      - apply H; try Progress.clean; try apply Progress.refl.
-        intros. focus § _ (_ [] _) § auto destruct.
+      - apply Sc; try assumption. apply Progress.refl.
+      - apply H; try Progress.solve.
+        intros y Vy Pxy. focus § _ (_ [] _) § auto destruct.
         apply IHfuel with (dir := dir); try assumption.
         apply Safety.continuation_weakening with (x := x); try assumption.
-        Progress.clean.
-      - apply H1; try assumption. apply Progress.refl.
-      - apply H; try Progress.clean; try apply Progress.refl.
-        intros. focus § _ (_ [] _) § auto destruct.
+        Progress.solve.
+      - apply Sc; try assumption. apply Progress.refl.
+      - apply H; try Progress.solve.
+        intros y Vy Pxy. focus § _ (_ [] _) § auto destruct.
         apply IHfuel with (dir := dir); try assumption.
         apply Safety.continuation_weakening with (x := x); try assumption.
-        Progress.clean.
-      - apply H; try Progress.clean; try apply Progress.refl.
-        intros. focus § _ (_ [] _) § auto destruct.
+        Progress.solve.
+      - apply H; try Progress.solve.
+        intros y Vy Pxy. focus § _ (_ [] _) § auto destruct.
         apply IHfuel with (dir := dir); try assumption.
         apply Safety.continuation_weakening with (x := x); try assumption.
-        Progress.clean.
-      - apply H1; try assumption. apply Progress.refl.
+        Progress.solve.
+      - apply Sc; try assumption. apply Progress.refl.
     Qed.
 
-    Lemma compileSubPattern: forall r dir rer, SafeMatcher dir | (compileSubPattern r rer dir).
+    Lemma compileSubPattern: forall r dir rer, SafeMatcher dir (compileSubPattern r rer dir).
     Proof.
-      induction r; cbn; intros;
+      induction r; cbn; intros dir rer x c Vx Sc;
       focus § _ (_ [] _) § auto destruct.
-      - apply H0.
-        + destruct dir; cbn in *; constructor; lia.
-        + inversion H. destruct dir; (constructor; cbn in *; solve [ assumption | constructor; cbn; lia ]).
+      - apply Sc.
+        + destruct dir; constructor; cbn in *; lia.
+        + inversion Vx. destruct dir; (constructor; cbn in *; solve [ assumption | constructor; cbn; lia ]).
       - apply Indexing.failure_kind in MatchEq_0.
         rewrite -> Indexing.failure_bounds in *.
-        hypotheses_reflector; destruct dir; cbn in *; lia.
-      - auto_specialize. apply IHr1HH0.
-      - auto_specialize. apply IHr2HH0.
+        unfold Valid in *. destruct dir; cbn in *; Zhelper; try lia.
+      - apply IHr1; assumption.
+      - apply IHr2; assumption.
       - apply Safety.repeatMatcher with (x := x) (dir := dir); try assumption.
         intros. apply IHr; try assumption.
       - intros.
         apply IHr1; try assumption.
-        intros. apply IHr2; try assumption.
+        intros y Vy Pxy. apply IHr2; try assumption.
         apply Safety.continuation_weakening with (x := x); assumption.
       - intros.
         apply IHr2 with (x := x); try assumption.
-        intros. apply IHr1; try assumption.
+        intros y Vy Pxy. apply IHr1; try assumption.
         apply Safety.continuation_weakening with (x := x); assumption.
       - apply IHr with (x := x); try assumption.
-        intros. focus § _ (_ [] _) § auto destruct.
-        + apply H0; Progress.clean.
+        intros y Vy Pxy. focus § _ (_ [] _) § auto destruct.
+        + apply Sc; Progress.solve.
         + focus § _ [] _ § auto destruct in MatchEq_;
-            destruct dir; try discriminate; inversion H2; inversion H7; spec_reflector Z.leb_spec0; lia.
-      - apply H0; Progress.clean. apply Progress.refl.
+            destruct dir; try discriminate; inversion Pxy; inversion H3; Zhelper; lia.
+      - apply Sc; Progress.solve.
       - rewrite <- MatchEq_0. apply IHr; try assumption.
         easy.
     Qed.
