MECMAR/tactics/Specialize.v
@@ -1,0 +1,16 @@
+Inductive Specialized {A B: Type} (a: A) (b: B) :=
+| AlreadySpecialized: Specialized a b.
+Ltac auto_specialize := repeat match goal with
+| [ a: _, b: _ |- _ ] => lazymatch goal with
+  | [ _: Specialized a b |- _ ] => fail
+  | [ |- _ ] =>
+    pose proof (AlreadySpecialized a b);
+    let H := fresh a b in
+    pose proof a as H;
+    specialize H with (1 := b)
+  end
+end.
+
+Ltac specialize_once := match goal with
+| [ H: _, H': _ |- _ ] => specialize H with (1 := H')
+end.
